cedar-lean/Cedar/Thm/Validation/Levels/CheckLevel.lean
@@ -75,8 +75,8 @@ inductive TypedExpr.AtLevel (env : TypeEnv) : TypedExpr → Nat → Prop where
     AtLevel env (.lit p ty) n
   | var (v : Var) (ty : CedarType) (n : Nat) :
     AtLevel env (.var v ty) n
-  | val (v : Value) (ty : CedarType) (n : Nat) :
-    AtLevel env (.val v ty) n
+  | val (v : TypedValue) (n : Nat) :
+    AtLevel env (.val v) n
   | ite (tx₁ tx₂ tx₃ : TypedExpr) (ty : CedarType) (n : Nat)
     (hl₁ : tx₁.AtLevel env n)
     (hl₂ : tx₂.AtLevel env n)
